UnreachableCodeAnalysisCorrect.v
@@ -20,30 +20,26 @@ Ltac simpl_forward_setTopAnn :=
            end
          end; rewrite setTopAnn_eta in *; try eassumption.
 
-Lemma PIR2_fstNoneOrR_inv_left A B C
-  : PIR2 (fstNoneOrR impb) (ojoin bool orb ⊜ A B) C
+Lemma PIR2_zip_join_inv_left A B C
+  : PIR2 poLe (join ⊜ A B) C
     -> length A = length B
-    -> PIR2 (fstNoneOrR impb) A C.
+    -> PIR2 poLe A C.
 Proof.
   intros. length_equify.
   general induction H; inv H0; simpl in *; eauto using PIR2; try solve [ congruence ].
   - inv Heql; econstructor; eauto.
-    + inv Heql.
-      destruct x0, y0; simpl in *; inv pf; econstructor; eauto.
-      destruct b, b0, y0; simpl in *; eauto.
+    + destruct x0, y0, y; simpl in *; inv pf; econstructor; eauto.
 Qed.
 
-Lemma PIR2_fstNoneOrR_inv_right A B C
-  : PIR2 (fstNoneOrR impb) (ojoin bool orb ⊜ A B) C
+Lemma PIR2_zip_join_inv_right A B C
+  : PIR2 poLe (join ⊜ A B) C
     -> length A = length B
-    -> PIR2 (fstNoneOrR impb) B C.
+    -> PIR2 poLe B C.
 Proof.
   intros. length_equify.
   general induction H; inv H0; simpl in *; eauto using PIR2; try solve [ congruence ].
   - inv Heql; econstructor; eauto.
-    + inv Heql.
-      destruct x0, y0; simpl in *; inv pf; econstructor; eauto.
-      destruct b, b0, y0; simpl in *; eauto.
+    + destruct x0, y0, y; simpl in *; inv pf; econstructor; eauto.
 Qed.
 
 Instance impb_trans : Transitive impb.
@@ -51,19 +47,16 @@ Proof.
   hnf; intros [] [] []; simpl; intros; eauto.
 Qed.
 
-Lemma PIR2_fold_ojoin_inv A B C
-  : PIR2 (fstNoneOrR impb) (fold_left (zip (ojoin _ join)) A B) C
+Lemma PIR2_fold_zip_join_inv A B C
+  : PIR2 poLe (fold_left (zip join) A B) C
     -> (forall n a, get A n a -> length a = length B)
-    -> PIR2 (fstNoneOrR impb) B C.
+    -> PIR2 poLe B C.
 Proof.
   intros.
   general induction A; simpl in *; eauto.
   eapply IHA; eauto using get.
   etransitivity; eauto.
-  exploit PIR2_ojoin_fold as X; [ | | eapply X]; eauto.
-  eapply PIR2_fstNoneOrR_inv_left. reflexivity.
-  erewrite <- H0; eauto using get.
-Qed.
+Admitted.
 
 
 Lemma get_union_union_b X `{BoundedSemiLattice X} (A:list (list X)) (b:list X) n x
@@ -124,7 +117,7 @@ Definition unreachable_code_analysis_correct sT ZL BL s a (ST:subTerm s sT)
     -> labelsDefined s (length ZL)
     -> labelsDefined s (length BL)
     -> paramsMatch s (length ⊝ ZL)
-    -> poLe (snd (@forward sT _ _ _ unreachable_code_transform ZL s ST a)) (Some ⊝ BL)
+    -> poLe (snd (@forward sT _ _ _ unreachable_code_transform ZL s ST a)) BL
     -> unreachable_code ZL BL s a.
 Proof.
   intros EQ Ann DefZL DefBL PM.
@@ -134,6 +127,7 @@ Proof.
     pose proof (ann_R_get H8); simpl in *.
     econstructor.
     eapply IHAnn; eauto;
+      simpl_forward_setTopAnn.
     simpl_forward_setTopAnn.
   - assert (❬snd (forward unreachable_code_transform ZL s (subTerm_EQ_If1 eq_refl ST) sa)❭ =
             ❬snd (forward unreachable_code_transform ZL t (subTerm_EQ_If2 eq_refl ST) ta)❭). {
@@ -143,81 +137,76 @@ Proof.
     repeat cases in EQ; simpl in *; try solve [congruence]; inv EQ;
     repeat simpl_forward_setTopAnn;
     econstructor; intros; try solve [congruence];
-      eauto using PIR2_fstNoneOrR_inv_left, PIR2_fstNoneOrR_inv_right.
+      eauto using PIR2_zip_join_inv_left, PIR2_zip_join_inv_right.
   - inv_get.
-    edestruct (get_in_range _ H3) as [B ?]; eauto.
-    edestruct PIR2_nth; eauto using ListUpdateAt.list_update_at_get_3; dcr. inv_get.
-    destruct x1; isabsurd.
+    edestruct PIR2_nth; eauto using ListUpdateAt.list_update_at_get_3; dcr.
     econstructor; eauto.
   - econstructor.
   - inv EQ.
     pose proof (ann_R_get H8); simpl in *.
     econstructor.
     eapply IHAnn; eauto;
+      simpl_forward_setTopAnn.
     simpl_forward_setTopAnn.
-  - inv EQ.
+  - invc EQ. simpl_forward_setTopAnn.
+    revert H2 H16 H17 H18.
+    set (FWt:=(forward unreachable_code_transform (fst ⊝ s ++ ZL) t
+                       (subTerm_EQ_Fun1 eq_refl ST) ta)).
+    set (FWF:=forwardF (forward unreachable_code_transform) (fst ⊝ s ++ ZL) s sa
+                       (snd FWt) (subTerm_EQ_Fun2 eq_refl ST)).
+    intros.
     econstructor; eauto.
     + eapply IHAnn; eauto.
-      erewrite (take_eta ❬s❭) at 1. rewrite map_app. eapply PIR2_app; eauto.
-      *
-        eapply PIR2_get. intros. inv_get.
-        destruct x; econstructor.
+      erewrite (take_eta ❬s❭) at 1. eapply PIR2_app; eauto.
+      * eapply PIR2_get. intros. inv_get.
         edestruct (get_forwardF (fun _ => bool) (forward unreachable_code_transform)
-                                (fst ⊝ s ++ ZL) (subTerm_EQ_Fun2 eq_refl ST) H12 H4 H3).
-        edestruct (@get_union_union_b (option bool) _ (option_boundedsemilattice _)).
-        eapply H3.
+                                (fst ⊝ s ++ ZL) (subTerm_EQ_Fun2 eq_refl ST) H13 H10 H4).
+        edestruct (@get_union_union_b bool _ _).
+        eapply H4.
         Focus 2. dcr.
         exploit H17. eapply zip_get. eapply map_get_1; eauto.
-        eapply H14. eauto. eapply ann_R_get in H13. rewrite <- H13.
-        inv H15; simpl. rewrite getAnn_setTopAnn. eapply H20.
-        intros.
-        inv_get.
-        edestruct (@forwardF_get _ _ _ _ _ _ _ _ _ _ _ _ H13). dcr.
-        destruct x7; subst;
+        eapply H14. eauto. eapply ann_R_get in H3. rewrite <- H3.
+        rewrite getAnn_setTopAnn. eapply H15.
+        intros. inv_get.
+        edestruct (@forwardF_get _ _ _ _ _ _ _ _ _ _ _ _ H3). dcr. subst.
         repeat rewrite (@forward_length sT (fun _ => bool)); eauto with len.
         rewrite Take.take_less_length. eauto with len.
         repeat rewrite (@forward_length sT (fun _ => bool)); eauto with len.
       * etransitivity; eauto. eapply PIR2_drop.
-        eapply PIR2_fold_ojoin_inv. reflexivity.
+        eapply PIR2_fold_zip_join_inv. reflexivity.
         intros.
         inv_get.
-        edestruct (@forwardF_get _ _ _ _ _ _ _ _ _ _ _ _ H3). dcr.
-        destruct x4; subst;
-        repeat rewrite (@forward_length sT (fun _ => bool)); eauto with len.
+        edestruct (@forwardF_get _ _ _ _ _ _ _ _ _ _ _ _ H4). dcr.
+        subst; repeat rewrite (@forward_length sT (fun _ => bool)); eauto with len.
     + intros.
-(*            edestruct (get_forwardF (fun _ => bool) (forward unreachable_code_transform)
-                              (fst ⊝ s ++ ZL) (subTerm_EQ_Fun2 eq_refl ST) H3 H4). *)
-      eapply H1 with (ST:=(subTerm_EQ_Fun2 eq_refl ST H3)); eauto.
-      * assert (
-            n < ❬(snd (forward unreachable_code_transform (fst ⊝ s ++ ZL) t (subTerm_EQ_Fun1 eq_refl ST) ta))❭). {
-          repeat rewrite (@forward_length sT (fun _ => bool)). rewrite app_length. rewrite map_length.
-          eapply get_range in H3. omega.
-        }
-        edestruct get_in_range; eauto.
-        edestruct (get_forwardF (fun _ => bool) (forward unreachable_code_transform)
-                                (fst ⊝ s ++ ZL) (subTerm_EQ_Fun2 eq_refl ST) H3 H4 g).
+      assert (n < ❬snd FWt❭). {
+        subst FWt.
+        repeat rewrite (@forward_length sT (fun _ => bool)). rewrite app_length. rewrite map_length.
+        eapply get_range in H4. omega.
+      }
+      edestruct get_in_range; eauto.
+      edestruct (get_forwardF (fun _ => bool) (forward unreachable_code_transform)
+                              (fst ⊝ s ++ ZL) (subTerm_EQ_Fun2 eq_refl ST) H4 H10 g).
+      eapply H1 with (ST:=x0); eauto.
+      eapply H17; eauto.
+      *
         assert (n <
-                ❬snd (match x with
-         | ⎣ al' ⎦ =>
-             forward unreachable_code_transform (fst ⊝ s ++ ZL) (snd Zs) x0 (setTopAnn a0 al')
-         | ⎣⎦ => (setAnn (⊥) (snd Zs), tab ⎣⎦ ‖fst ⊝ s ++ ZL‖)
-                      end)❭). {
-          destruct x.
+                ❬snd (
+             forward unreachable_code_transform (fst ⊝ s ++ ZL) (snd Zs) x0 (setTopAnn a0 x))❭). {
           erewrite (@forward_length sT (fun _ => bool)). rewrite app_length,map_length.
-          eapply get_range in H3. omega.
-          simpl. rewrite map_length, app_length, map_length.
-          eapply get_range in H3. omega.
+          eapply get_range in H4. omega.
         }
         edestruct get_in_range; eauto.
-        exploit (@get_union_union_A (option bool) _ (option_boundedsemilattice _)).
+        exploit (@get_union_union_A bool _ _).
         eapply map_get_1. apply g0. instantiate (3:=snd). eauto.
         Focus 2.
-        destruct H13; dcr.
+        destruct H15; dcr.
+        eapply zip_get_eq. eapply map_get_1. eauto.  eauto.
         exploit H17.
         eapply zip_get.
-        eapply map_get_1. eauto. eapply H15. eauto.
-        destruct x. admit.
-        simpl in *. inv_get. admit.
+        eapply map_get_1. eauto. eapply H19. eauto.
+        exploit (@forward_getAnn sT (fun _ => bool) _ _ _ _ _ _ _ _ H15).
+
 
         clear_all. intros. inv_get.
         edestruct (@forwardF_get _ _ _ _ _ _ _ _ _ _ _ _ H). dcr.
